Show that if n is a positive integer, then

$1+2 + ⋯ + n = \frac{n(n + 1)}{2}$

Base case:
Must show that $P(n)=1+2 + ⋯ + n = \frac{n(n + 1)}{2}$

$P(1)=1=\frac{1(1 + 1)}{2}$

$P(1)=1=\frac{2}{2}$

$P(1)=1=1$ its true

INDUCTIVE STEP: For the inductive hypothesis we assume that P(k) holds for an arbitrary positive integer k. 

$P(k)=1+2 + ⋯ + k = \frac{k(k + 1)}{2}$

then we have to show for 

$P(k+1)=1+2 + ⋯ + k + (k+1) = \frac{(k+1)((k+1) + 1)}{2}=\frac{(k+1)(k+2)}{2}$

We can use definition that:

$P(k)=1+2 + ⋯ + k = \frac{k(k + 1)}{2}$

Because of the assumption:

$P(k+1)=\frac{k(k + 1)}{2} + (k+1) =\frac{(k+1)(k+2)}{2}$

Obtain same denominator

$P(k+1)=\frac{k(k + 1)+2(k+1)}{2} =\frac{(k+1)(k+2)}{2}$

# $\frac{k(k + 1)+2(k+1)}{2}$

Factor out k+1

 $\frac{(k+1)(k+2)}{2}$
 
Put 1 out of parenthesis

 $\frac{(k+1)((k+1)+1)}{2}= \frac{(k+1)((k+1)+1)}{2}$
 
 Proof ended


